more contexts infrastructure and ctx interp

theories/contexts.v
@@ -1,359 +1,54 @@
-(** Properties of Wasm label/evaluation contexts *)
+(** Inductively defined contexts extract to code that run very poorly. This alternative defines an
+    additional context stack to replace the inductive definition, since the evaluation context tree is
+    always guaranteed to be linear. **)
 
 From mathcomp Require Import ssreflect ssrfun ssrnat ssrbool eqtype seq.
-From Coq Require Import Program.Equality NArith ZArith.
-From Wasm Require Export common operations datatypes_properties properties.
+From Coq Require Import Program NArith ZArith Wf_nat.
+From Wasm Require Export common operations datatypes_properties properties opsem.
+Require Import FunInd Recdef.
 
 Set Implicit Arguments.
 Unset Strict Implicit.
 Unset Printing Implicit Defensive.
 
-
-(** Decidable equality of lholed without pulling in unnecessary 
-    equality axioms **)
-Section lholed_eqdec.
-
-Definition lholed_cast {k k'} (lh: lholed k) (Heq: k = k'): lholed k' :=
-  eq_rect k lholed lh k' Heq.
-
-(* Some combinations of theorem from standard library should give these as well,
-   but it's not clear which ones are axiom free *)
-Theorem nat_eqdec_refl: forall k, Nat.eq_dec k k = left (erefl k).
-Proof.
-  elim => //=.
-  move => k IH.
-  by rewrite IH.
-Defined.
-
-Definition nat_eqdec_canon k k' (H: k = k') : k = k' :=
-  match (Nat.eq_dec k k') with
-  | left e => e
-  | right ne => False_ind _ (ne H)
-  end.
-
-Theorem nat_eqdec_aux: forall (k: nat) (H: k = k), H = nat_eqdec_canon H.
-Proof.
-  move => k H.
-  case H.
-  unfold nat_eqdec_canon.
-  by rewrite nat_eqdec_refl.
-Defined.
-
-Theorem nat_eqdec_unique: forall (k: nat) (H: k = k), H = erefl k.
-Proof.
-  move => k H.
-  rewrite (nat_eqdec_aux H).
-  unfold nat_eqdec_canon.
-  by rewrite nat_eqdec_refl.
-Defined.
-
-Theorem lh_cast_eq {k} (lh: lholed k) (Heq: k = k):
-  @lholed_cast k k lh Heq = lh.
-Proof.
-  by rewrite (nat_eqdec_unique Heq).
-Qed.
-
-Ltac decide_eq_arg x y :=
-  let Heq := fresh "Heq" in
-  let Hcontra := fresh "Hcontra" in
-  destruct (x == y) eqn:Heq; move/eqP in Heq; subst; last by right; move => Hcontra; injection Hcontra.
-
-Definition lh_case: forall n (P: lholed n -> Type),
-    (forall (H: 0 = n) vs es, P (lholed_cast (LH_base vs es) H)) ->
-    (forall n' (H: S n' = n) vs k es (lh: lholed n') es', P (lholed_cast (LH_rec vs k es lh es') H)) ->
-    (forall (lh: lholed n), P lh).
-Proof.
-  move => n P H0 Hrec lh.
-  destruct lh as [lvs les | n lvs k les lh les'].
-  - by specialize (H0 (erefl 0) lvs les).
-  - by specialize (Hrec _ (erefl (S n)) lvs k les lh les'). 
-Defined.
-
-(* Decidable equality of lholed without eq_rect_eq *)
-Definition lholed_eq_dec : forall k (lh1 lh2 : lholed k), {lh1 = lh2} + {lh1 <> lh2}.
-Proof.
-  elim.
-  {
-    move => lh1.
-    eapply lh_case; last done.
-    move => H vs es; rewrite lh_cast_eq.
-    move: lh1.
-    eapply lh_case; last done.
-    move => H' vs' es'; rewrite lh_cast_eq.
-    decide_eq_arg vs' vs.
-    decide_eq_arg es' es.
-    by left.
-  }
-  {
-    move => n IH lh.
-    eapply lh_case; first done.
-    move => n1 H1 vs1 k1 es1 lh1 es1'; injection H1 as ->; rewrite lh_cast_eq.
-    move: lh.
-    eapply lh_case; first done.
-    move => n2 H2 vs2 k2 es2 lh2 es2'; injection H2 as ->; rewrite lh_cast_eq.
-    decide_eq_arg vs2 vs1.
-    decide_eq_arg k2 k1.
-    decide_eq_arg es2 es1.
-    decide_eq_arg es2' es1'.
-    destruct (IH lh1 lh2) as [ | Hneq]; subst; first by left.
-    right. move => Hcontra; apply Hneq.
-    clear - Hcontra.
-    inversion Hcontra.
-    (* This one is axiom free *)
-    apply Eqdep_dec.inj_pair2_eq_dec in H0 => //.
-    decide equality.
-  }
-Defined.
-
-Definition lholed_eqb {k} (v1 v2: lholed k) : bool := lholed_eq_dec v1 v2.
-
-Definition eqlholedP {k} :=
-  eq_dec_Equality_axiom (@lholed_eq_dec k).
-
-Canonical Structure lholed_eqMixin {k} := EqMixin (@eqlholedP k).
-Canonical Structure lholed_eqType {k} := Eval hnf in EqType (@lholed k) (@lholed_eqMixin k).
-
-End lholed_eqdec.
-
-Lemma lfilled_not_nil {k}: forall (lh: lholed k) es es', lfill lh es = es' -> es <> [::] -> es' <> [::].
-Proof.
-  elim => /=.
-  { move => vs ? es ? <- ?.
-    by destruct es, vs => //.
-  }
-  { move => k' vs n es lh' IH vs' ?? <- ?.
-    by destruct vs.
-  }
-Qed.
-
-(** label context arithmetics **)
-Fixpoint empty_vs_base {k} (lh: lholed k) : bool :=
-  match lh with
-  | LH_base [::] _ => true
-  | LH_rec _ _ _ _ lh _ => empty_vs_base lh
-  | _ => false
-  end.
-
-Fixpoint lh_push_base_vs {k} (lh: lholed k) rvs: lholed k :=
-  match lh with
-  | LH_base vs es => LH_base (vs ++ rvs) es
-  | LH_rec _ vs n es lh' es' =>
-      let lh_pushed := lh_push_base_vs lh' rvs in
-      LH_rec vs n es lh_pushed es'
-  end.
-
-Definition lh_push_front_vs {k} vcs (lh: lholed k): lholed k :=
-  match lh with
-  | LH_base vs es => LH_base (vcs ++ vs) es
-  | LH_rec _ vs n es lh' es' => LH_rec (vcs ++ vs) n es lh' es'
-  end.
-
-Definition lh_drop_vs {k} l (lh: lholed k): lholed k :=
-  match lh with
-  | LH_base vs es => LH_base (drop l vs) es
-  | LH_rec _ vs n es lh' es' => LH_rec (drop l vs) n es lh' es'
-  end.
-
-Definition lh_drop_vs_o {k} l (lh: lholed k): option (lholed k) :=
-  match lh with
-  | LH_base vs es =>
-      if l <= length vs then Some (LH_base (drop l vs) es)
-      else None
-  | LH_rec _ vs n es lh' es' =>
-      if l <= length vs then Some (LH_rec (drop l vs) n es lh' es')
-      else None
-  end.
-
-Definition lh_push_back_es {k} es0 (lh: lholed k): lholed k :=
-  match lh with
-  | LH_base vs es => LH_base vs (es ++ es0)
-  | LH_rec _ vs n es lh' es' => LH_rec vs n es lh' (es' ++ es0)
-  end.
-
-Lemma lfill_push_base_vs {k} : forall (lh: lholed k) vs ves es,
-  ves = v_to_e_list vs ->
-  lfill lh (ves ++ es) = lfill (lh_push_base_vs lh vs) es.
-Proof.
-  induction lh as [vs es | ? vs n es lh' IH es'']; intros rvs vcs e ->; simpl in *.
-  - by rewrite/v_to_e_list map_cat -catA -catA.
-  - do 3 f_equal.
-    by eapply IH; eauto.
-Qed.
-
-Lemma lfill_push_base_vs' {k}: forall (lh: lholed k) vs ves es l,
-    ves = v_to_e_list vs ->
-    length ves >= l ->
-    lfill lh (ves ++ es) = lfill (lh_push_base_vs lh (take (length ves - l) vs)) ((drop (length ves - l) ves) ++ es).
-Proof.
-  move => lh vs ves es l Hves Hlen.
-  rewrite -(cat_take_drop (length ves - l) ves) -catA.
-  erewrite <-lfill_push_base_vs; eauto.
-  subst.
-  repeat rewrite catA cat_take_drop v_to_e_take.
-  by rewrite length_is_size v_to_e_size catA cat_take_drop.
-Qed.
-
-Lemma lfill_push_front_vs {k} : forall (lh: lholed k) vs es LI,
-    lfill lh es = LI ->
-    lfill (lh_push_front_vs vs lh) es = v_to_e_list vs ++ LI.
-Proof.
-  move => lh vs es LI <-.
-  by destruct lh => //=; rewrite - v_to_e_cat -catA.
-Qed.
-
-Lemma lfill_drop_impl {k}: forall (lh: lholed k) ves e es LI,
-    const_list ves ->
-    is_const e = false ->
-    lfill lh (e :: es) = ves ++ LI ->
-    lh_drop_vs_o (length ves) lh = Some (lh_drop_vs (length ves) lh).
-Proof.
-  move => lh ves e es LI Hconst Hnconst Heq.
-  destruct lh; simpl in * => //.
-  all: apply es_split_by_non_const in Heq; eauto; (try by apply v_to_e_const); destruct Heq as [? Heq].
-  all: replace (length ves <= length l) with true; (apply f_equal with (f := @size administrative_instruction) in Heq; rewrite size_cat v_to_e_size in Heq; simpl in Heq; repeat rewrite length_is_size; by lias).
-Qed.
-  
-Lemma lfill_drop_vs {k}: forall (lh: lholed k) ves e es LI,
-    const_list ves ->
-    is_const e = false ->
-    lfill lh (e :: es) = ves ++ LI ->
-    lfill (lh_drop_vs (length ves) lh) (e :: es) = LI.
-Proof.
-  move => lh ves e es LI Hconst Hnconst Heq.
-  destruct lh; simpl in * => //.
-  all: specialize (es_split_by_non_const Heq) as Heq2; destruct Heq2 as [xs Heq2]; eauto; (try by apply v_to_e_const).
-  all: rewrite -(cat_take_drop (length ves) l) -v_to_e_cat -catA in Heq.
-  all: apply concat_cancel_first_n in Heq; last by rewrite v_to_e_size size_take; apply f_equal with (f := size) in Heq2; rewrite v_to_e_size size_cat in Heq2; rewrite length_is_size; destruct (size ves < size l) eqn:?; lias.
-  all: move/andP in Heq; destruct Heq as [Heqves HeqLI]; move/eqP in Heqves; by move/eqP in HeqLI.
-Qed.
-
-Lemma lfill_push_back_es {k}: forall (lh: lholed k) es es0,
-    lfill (lh_push_back_es es0 lh) es = lfill lh es ++ es0.
-Proof.
-  move => lh es es0.
-  destruct lh; simpl in * => //; by repeat rewrite -catA => //.
-Qed.
-
-
-Fixpoint ai_gen_measure (e: administrative_instruction) : nat :=
-  match e with
-  | AI_label _ _ es => 1 + List.list_max (map ai_gen_measure es)
-  | _ => 0
-  end.
-
-Definition ais_gen_measure (LI: list administrative_instruction) : nat :=
-  List.list_max (map ai_gen_measure LI).
-
-Lemma lfill_const: forall k (lh: lholed k) e lf,
-    const_list lf ->
-    lfill lh [::e] = lf ->
-    {vs & {es & {Heq: k = 0 & lholed_cast lh Heq = (LH_base vs es) /\ lf = v_to_e_list vs ++ [::e] ++ es}}}.
-Proof.
-  move => k lh.
-  destruct lh as [lvs les | k lvs j lces lh les] => //.
-  - move => e lf /=Hconst Hlf.
-    subst.
-    apply const_list_split in Hconst as [_ Hconst].
-    simpl in Hconst.
-    move/andP in Hconst; destruct Hconst as [? Hconst].
-    destruct e as [b | | | |] => //; destruct b => //.
-    exists lvs, les, (Logic.eq_refl 0).
-    by split => //.
-  - move => e lf Hconst Hlf. subst.
-    exfalso.
-    apply const_list_split in Hconst as [_ Hconst].
-    by simpl in Hconst.
-Qed.
-
-Lemma const_seq_factorise (fe: nat -> administrative_instruction) (ves: list administrative_instruction):
-  {vs & {es & ves = v_to_e_list vs ++ [::fe 0] ++ es}} + {forall vs es, ves <> v_to_e_list vs ++ [::fe 0] ++ es}.
-Proof.
-  move: fe.
-  induction ves as [ | e ves']; move => fe; first by right; destruct vs => //.
-  destruct (e == fe 0) eqn:H; move/eqP in H.
-  - subst.
-    left; by exists nil, ves'.
-  - destruct (is_const e) eqn:Hconst.
-    { destruct e as [ b | | | |] => //; destruct b => //.
-      destruct (IHves' fe) as [[vs [es ->]] | Hcontra]; first by left; exists (v :: vs), es.
-      right; move => vs es Heq.
-      destruct vs as [| v0 vs'] => //; simpl in *; first by inversion Heq.
-      apply (Hcontra vs' es) => /=; by inversion Heq.
-    }
-    { right; move => vs es Heq.
-      destruct vs as [| v0 vs'] => //; simpl in *; by inversion Heq; subst.
-    }
-Qed.
-    
-Definition lf_decide fe es: Type := {n & {lh: lholed n | lfill lh [::fe n] = es}} + {forall n (lh: lholed n), lfill lh [::fe n] <> es}.
-
-Definition lfill_factorise_aux (fe: nat -> administrative_instruction) (es: list administrative_instruction) (Hrec: forall fe es', (ais_gen_measure es' < ais_gen_measure es)%coq_nat -> lf_decide fe es'):
-    lf_decide fe es.
-Proof.
-  (* First, decide if lfill0 hold *)
-  destruct (const_seq_factorise fe es) as [[vs' [es'' Heq]] | Hcontra]; first by left; exists 0, (LH_base vs' es'').
-  (* If not, then look at the top of instruction stack *)
-  destruct (split_vals_e es) as [vs es'] eqn:Hsplit.
-  destruct es' as [| e es'].
-  (* Instruction stack is empty *)
-  - right. move => n lh Hlf.
-    apply split_vals_inv in Hsplit as ->; rewrite cats0 in Hlf.
-    rewrite cats0 in Hcontra.
-    apply lfill_const in Hlf; last by apply v_to_e_const.
-    destruct Hlf as [vs' [es [-> [? Heq]]]]; simpl in *; subst.
-    by apply Hcontra in Heq.
-  - specialize (split_vals_nconst Hsplit) as Hnconst.
-    apply split_vals_inv in Hsplit as ->.
-    destruct e as [ | | | j lvs les |].
-    4: {
-      destruct (Hrec (fun n => fe (S n)) les) as [IH | IH] => /=.
-      (* measure *)
-      {
-        unfold ais_gen_measure.
-        rewrite - cat1s map_cat map_cat cat_app cat_app.
-        repeat rewrite List.list_max_app => /=.
-        destruct (List.list_max (map ai_gen_measure es')); by lias.
-      }
-      { destruct IH as [n' [lh' Hlf]].
-        left.
-        exists (S n'), (LH_rec vs j lvs lh' es') => /=.
-        by rewrite Hlf.
-      }
-      { right. move => n lh Hlf.
-        destruct lh as [lvs' les' | n' lvs' les' lh' les'']; simpl in *; first by apply (Hcontra lvs' les').
-        apply const_list_concat_inv in Hlf as [Heq [Heqlab <-]] => //; try by apply v_to_e_const.
-        apply v_to_e_inj in Heq as ->.
-        injection Heqlab as <- <- <-.
-        by eapply IH.
-      }
-    }
-    all: right; move => n' lh Hlf; destruct lh as [lvs' les' | n' lvs' les' lh' les'']; simpl in *; (try by apply (Hcontra lvs' les')); apply const_list_concat_inv in Hlf as [Heq [Heqlab <-]] => //; by apply v_to_e_const.
-Defined.
-
-Program Fixpoint lfill_factorise fe es {measure (ais_gen_measure es)} :=
-  @lfill_factorise_aux fe es lfill_factorise.
-
-
-(** Inductively defined contexts extract to code that run very poorly. This alternative defines an
-    additional context stack to replace the inductive definition, since the evaluation context tree is
-    always guaranteed to be linear. **)
 Module EvalContext.
+
+Parameter host_function: eqType.
+
+Parameter host_instance: host host_function.
+
+#[local]
+Definition reduce := @reduce host_function host_instance.
 
 Class eval_ctx (ctx_t: Type): Type :=
   {
-    ctx_fill: ctx_t -> list administrative_instruction -> list administrative_instruction;
+    ctx_fill: list administrative_instruction -> ctx_t -> list administrative_instruction;
+    ctx_frame_mask: ctx_t -> frame -> frame;
+    ctx_frame_cond: ctx_t -> frame -> frame -> Prop;
+    ctx_reduce: forall (ctx: ctx_t) hs s f es hs' s' f' es',
+      ctx_frame_cond ctx f f' ->
+      reduce hs s (ctx_frame_mask ctx f) es hs' s' (ctx_frame_mask ctx f') es' ->
+      reduce hs s f (ctx_fill es ctx) hs' s' f' (ctx_fill es' ctx);
   }.
 
-Notation "ctx [[ es ]]" := (ctx_fill ctx es) (at level 5).
+Notation "ctx ⦃ es ⦄" := (ctx_fill es ctx) (at level 1).
 
-(* Sequence context: vs ++ [_] ++ es. This is only used in the base level *)
+Definition fmask0 {T1 T2: Type} := (fun (_: T1) => @id T2).
+
+Definition fcond0 {T1 T2 T3: Type} := (fun (_: T1) (_: T2) (_: T3) => True).
+
+(* Sequence context: rev vs ++ [_] ++ es. This is only used in the base level *)
 Definition seq_ctx : Type := (list value) * (list administrative_instruction).
 
-#[export]
+#[refine, export]
 Instance seq_ctx_eval : eval_ctx seq_ctx :=
-  {| ctx_fill := (fun ctx es => (v_to_e_list (fst ctx) ++ es ++ (snd ctx))) |}.
+  {| ctx_fill := (fun es ctx => (vs_to_es (fst ctx) ++ es ++ snd ctx)); ctx_frame_mask := fmask0; ctx_frame_cond := fcond0 |}.
+Proof.
+  move => ctx hs s f es hs' s' f' es' _ Hred.
+  by eapply r_label with (lh := LH_base (rev (fst ctx)) (snd ctx)); eauto.
+Defined.
 
-(* Label context: LC_val ++ [::AI_label LC_arity LC_cont [_]) ++ LC_post; can be nested *)
+(* Label context: rev LC_val ++ [::AI_label LC_arity LC_cont [_]) ++ LC_post; can be nested *)
 Record label_ctx: Type :=
   { LC_val: list value;
     LC_arity: nat;
@@ -361,21 +56,17 @@ Record label_ctx: Type :=
     LC_post: list administrative_instruction;
   }.
 
-Definition label_ctx_fill := (fun ctx es => (v_to_e_list (LC_val ctx) ++ [::AI_label (LC_arity ctx) (LC_cont ctx) es] ++ LC_post ctx)).
+Definition label_ctx_fill := (fun es ctx => (vs_to_es (LC_val ctx) ++ [::AI_label (LC_arity ctx) (LC_cont ctx) es] ++ (LC_post ctx))).
 
-#[export]
+#[refine, export]
 Instance label_ctx_eval: eval_ctx label_ctx :=
-  {| ctx_fill := label_ctx_fill |}.
+  {| ctx_fill := label_ctx_fill; ctx_frame_mask := fmask0; ctx_frame_cond := fcond0 |}.
+Proof.
+  move => [lvs lk lces les] hs s f es hs' s' f' es' _ Hred.
+  eapply r_label with (lh := LH_rec (rev lvs) lk lces (LH_base nil nil) les); eauto => //; by rewrite /label_ctx_fill /= cats0.
+Defined.
 
-Canonical label_ctx_eval.
-
-#[export]
-Instance list_ctx_eval {T: Type} (f: eval_ctx T): eval_ctx (list T) :=
-  {| ctx_fill := (fun ctxs es => foldr f.(ctx_fill) es ctxs) |}.
-
-Definition label_list_ctx: Type := list label_ctx.
-
-(* Frame context: FC_val ++ [::AI_local FC_arity FC_frame [_]) ++ FC_post *)
+(* Frame context: rev FC_val ++ [::AI_local FC_arity FC_frame [_]) ++ FC_post *)
 Record frame_ctx: Type :=
   { FC_val: list value;
     FC_arity: nat;
@@ -383,24 +74,510 @@ Record frame_ctx: Type :=
     FC_post: list administrative_instruction;
   }.
 
-#[export]
+#[refine, export]
 Instance frame_ctx_eval: eval_ctx frame_ctx :=
-  {| ctx_fill := (fun ctx es => (v_to_e_list (FC_val ctx) ++ [::AI_local (FC_arity ctx) (FC_frame ctx) es] ++ FC_post ctx)) |}.
+  {| ctx_fill := (fun es ctx => (vs_to_es (FC_val ctx) ++ [::AI_local (FC_arity ctx) (FC_frame ctx) es] ++ (FC_post ctx)));
+    ctx_frame_mask := (fun ctx _ => ctx.(FC_frame));
+    ctx_frame_cond := (fun _ f1 f2 => f1 = f2);
+  |}.
+Proof.
+  move => [lvs lk lf les] hs s f es hs' s' f' es' /= <- Hred /=.
+  eapply r_label with (lh := LH_base (rev lvs) les); eauto => //=; try by rewrite -cat1s.
+  by apply r_local.
+Defined.
 
-Definition closure_ctx : Type := (option frame_ctx) * label_ctx * seq_ctx.
-
-Definition closure_ctx_fill (cc: closure_ctx) es :=
-  match cc with
-  | (Some fc, lc, sc) => fc [[ lc [[ sc [[ es ]] ]] ]]
-  | (None, lc, sc) => lc [[ sc [[ es ]] ]]
+Fixpoint ctx_frame_cond_list {T: Type} {ctx_p: eval_ctx T} (ctxs: list T) (f1 f2: frame): Prop :=
+  match ctxs with
+  | nil => True
+  | ctx :: ctxs' =>
+      ctx_p.(ctx_frame_cond) ctx (foldr ctx_p.(ctx_frame_mask) f1 ctxs') (foldr ctx_p.(ctx_frame_mask) f2 ctxs') /\
+      ctx_frame_cond_list ctxs' f1 f2
   end.
 
-#[export]
-Instance closure_ctx_eval: eval_ctx closure_ctx :=
-  {| ctx_fill := closure_ctx_fill |}.
+(* A general instance for lists of evaluation contexts *)
+#[refine, export]
+Instance list_ctx_eval {T: Type} (ctx_p: eval_ctx T): eval_ctx (list T) :=
+  {| ctx_fill := (fun es ctxs => foldl ctx_p.(ctx_fill) es ctxs);
+    ctx_frame_mask := (fun ctxs f => foldr ctx_p.(ctx_frame_mask) f ctxs);
+    ctx_frame_cond := ctx_frame_cond_list
+  |}.
+Proof.
+  elim => //.
+  move => ctx ctxs' IH hs s f es hs' s' f' es' /=[Hcond Hconds] /=Hred /=.
+  apply ctx_p.(ctx_reduce) in Hred => //=.
+  by apply IH in Hred => //=.
+Defined.
 
-(* A configuration is now represented as (S; F; ctx [[ e ]]), with the hole holding at most one instruction.
-   The hole is allowed to be empty (in which case the inner context is then exitted. *)
-Definition cfg_tuple_ctx {host_function: eqType}: Type := (store_record host_function) * frame * list closure_ctx * option administrative_instruction.
+Lemma ctx_frame_cond_list_label: forall (lcs: list label_ctx) f,
+  ctx_frame_cond_list lcs f f.
+Proof.
+  by elim.
+Qed.
+
+Lemma ctx_frame_cond_list_frame: forall (lcs: list frame_ctx) f,
+  ctx_frame_cond_list lcs f f.
+Proof.
+  by elim.
+Qed.
+
+Definition closure_ctx : Type := frame_ctx * list label_ctx.
+
+Definition closure_ctx_fill es (cc: closure_ctx):=
+  match cc with
+  | (fc, lc) => fc ⦃ lc ⦃ es ⦄ ⦄
+  end.
+
+Lemma foldr_id {T1 T2: Type}: forall (l: list T1) (x: T2),
+    foldr (fun _ => id) x l = x.
+Proof.
+  by elim.
+Qed.
+  
+(* Simpler instances for label and frame contexts *)
+#[refine, export]
+Instance list_label_ctx_eval : eval_ctx (list label_ctx) :=
+  {| ctx_fill := (@list_ctx_eval label_ctx _).(ctx_fill);
+    ctx_frame_mask := fmask0;
+    ctx_frame_cond := fcond0;
+    |}.
+Proof.
+  elim => //.
+  move => [lvs lk lces les] ctxs' IH hs s f es hs' s' f' es' _ Hred /=.
+  rewrite /fmask0 in Hred.
+  rewrite /label_ctx_fill /=.
+  apply IH => //.
+  rewrite /fmask0.
+  eapply r_label with (lh := LH_rec (rev lvs) lk lces (LH_base nil nil) les); eauto => //; by rewrite /label_ctx_fill /= cats0.
+Defined.
+
+#[refine, export]
+Instance list_frame_ctx_eval : eval_ctx (list frame_ctx) :=
+  {| ctx_fill := (@list_ctx_eval frame_ctx _).(ctx_fill);
+    ctx_frame_mask := (fun ctxs f0 =>
+                         match ctxs with
+                         | nil => f0
+                         | ctx :: ctxs' => ctx.(FC_frame)
+                         end);
+    ctx_frame_cond := (fun _ f1 f2 => f1 = f2);
+    |}.
+Proof.
+  case => //.
+  move => ctx ctxs'; move: ctxs' ctx.
+  elim => //.
+  - move => [lvs lk lf les] hs s f es hs' s' f' es' <- /=Hred /=.
+    eapply r_label with (lh := LH_base (rev lvs) les); eauto => //=; try by rewrite -cat1s.
+    by apply r_local.
+  - move => ctx ctxs' IH [lvs lk lf les] hs s f es hs' s' f' es' <- /=Hred.
+    apply IH => //=.
+    eapply r_label with (lh := LH_base (rev lvs) les); eauto => //=; try by rewrite -cat1s.
+    by apply r_local.
+Defined.
+
+#[refine, export]
+Instance closure_ctx_eval: eval_ctx closure_ctx :=
+  {| ctx_fill := closure_ctx_fill;
+     ctx_frame_mask := (fun '(fc, lc) _ => fc.(FC_frame));
+     ctx_frame_cond := (fun _ f1 f2 => f1 = f2);
+  |}.
+Proof.
+  move => [fc lcs] hs s f es hs' s' f' es' <- Hred.
+  apply (@ctx_reduce _ _ fc) => //.
+  apply (@ctx_reduce _ _ lcs) => /=; first by apply ctx_frame_cond_list_label.
+  by rewrite foldr_id.
+Defined.
+
+#[refine, export]
+Instance list_closure_ctx_eval : eval_ctx (list closure_ctx) :=
+  {| ctx_fill := (@list_ctx_eval closure_ctx _).(ctx_fill);
+    ctx_frame_mask := (fun ctxs f0 =>
+                         match ctxs with
+                         | nil => f0
+                         | (fc, lcs) :: ctxs' => fc.(FC_frame)
+                         end);
+    ctx_frame_cond := (fun _ f1 f2 => f1 = f2);
+    |}.
+Proof.
+  case => //.
+  move => ctx ctxs'; move: ctxs' ctx.
+  elim => //.
+  - move => [[lvs lk lf les] lcs] hs s f es hs' s' f' es' <- /=Hred /=.
+    eapply r_label with (lh := LH_base (rev lvs) les); eauto => //=; try by rewrite -cat1s.
+    apply r_local.
+    by apply (list_label_ctx_eval.(ctx_reduce)).
+  - move => ctx ctxs' IH [[lvs lk lf les] lcs] hs s f es hs' s' f' es' <- /=Hred.
+    apply IH => //=.
+    eapply r_label with (lh := LH_base (rev lvs) les); eauto => //=; try by rewrite -cat1s.
+    apply r_local.
+    by apply (list_label_ctx_eval.(ctx_reduce)).
+Defined.
+
+(* A configuration is now represented as (S; ctxs ⦃ sc ⦃ option e ⦄ ⦄), with the hole holding at most one instruction which needs to be non-constant.
+   Note that no frame is held in the tuple, since all frames should have been pushed into the local contexts.
+   The contexts are represented in a reversed stack-like structure: the head of each list is the innermost context.
+   The hole is allowed to be empty (in which case the inner context is then exitted on the next step). *)
+Definition cfg_tuple_ctx {host_function: eqType}: Type := (store_record host_function) * list closure_ctx * seq_ctx * option administrative_instruction.
+
+Definition valid_hole (e: administrative_instruction) : bool :=
+  match e with
+  | AI_label _ _ _ => false
+  | AI_local _ _ _ => false
+  | AI_basic (BI_const _) => false
+  | _ => true
+  end.
+
+Definition valid_split (sc: seq_ctx) oe: bool :=
+  match oe with
+  | Some e => valid_hole e
+  | None => snd sc == nil
+  end.
+
+(* The canonical form of a context config tuple: 
+   - The ves split has to be valid;
+   - The closure can only be empty if the entire instruction is already a value. 
+*)
+Definition valid_cfg_ctx {host_function: eqType} (cfg: @cfg_tuple_ctx host_function) : Prop :=
+  match cfg with
+  | (_, cc, sc, oe) =>
+      (cc = nil -> oe = None /\ snd sc = nil) /\ valid_split sc oe
+  end.
+
+Definition olist {T: Type} (ot: option T) : list T :=
+  match ot with
+  | Some t => [::t]
+  | None => nil
+  end.
+
+Fixpoint ai_measure (e: administrative_instruction) : nat :=
+  match e with
+  | AI_label _ _ es => 1 + List.list_sum (map ai_measure es)
+  | AI_local _ _ es => 1 + List.list_sum (map ai_measure es)
+  | _ => 1
+  end.
+
+Definition ais_measure (LI: list administrative_instruction) : nat :=
+  List.list_sum (map ai_measure LI).
+
+Lemma ais_measure_cat: forall l1 l2,
+    ais_measure (l1 ++ l2) = ais_measure l1 + ais_measure l2.
+Proof.
+  move => l1 l2.
+  unfold ais_measure.
+  by rewrite map_cat cat_app List.list_sum_app.
+Qed.
+
+Lemma ais_measure_cons: forall x l,
+    ais_measure (x :: l) = ai_measure x + ais_measure l.
+Proof.
+  done.
+Qed.
+
+(*
+Definition ai_rect' (P: administrative_instruction -> Type)
+  (e : administrative_instruction)
+  (f_basic : forall b : basic_instruction, P (AI_basic b)) 
+  (f_trap : P AI_trap)
+  (f_invoke : forall addr : funcaddr, P (AI_invoke addr))
+  (f_label : forall (n : nat) (ces es : seq administrative_instruction), ais_measure es < ai_measure e -> P (AI_label n ces es))
+  (f_local : forall (n : nat) (f : frame) (es : seq administrative_instruction), ais_measure es < ai_measure e -> P (AI_local n f es))
+  : (P e).
+Proof.
+  destruct e as
+    [ b
+    |
+    | addr
+    | n ces es
+    | n f es
+    ].
+  - exact (f_basic b).
+  - exact (f_trap).
+  - exact (f_invoke addr).
+  - by apply f_label.
+  - by apply f_local.
+Defined.
+*)
+
+Definition empty_instance := Build_instance nil nil nil nil nil.
+
+Definition empty_frame := Build_frame nil empty_instance.
+
+(* Placeholder so that ctx_decompose can be useful for instructions without the outer frame, although not the
+   intended purpose *)
+Definition empty_frame_ctx := Build_frame_ctx nil 0 empty_frame nil.
+
+(* Tail recursive version of split_vals_e, also producing the reversed vs list used in the contexts *)
+Fixpoint split_vals'_aux (ves: list administrative_instruction) (acc: list value) : (list value) * (list administrative_instruction) :=
+  match ves with
+  | nil => (acc, nil)
+  | e :: ves' =>
+      match e_to_v_opt e with
+      | Some v => split_vals'_aux ves' (v :: acc)
+      | None => (acc, ves)
+      end
+  end.
+
+Definition split_vals' ves := split_vals'_aux ves nil.
+
+Lemma split_vals'_aux_impl: forall ves acc vs es,
+    split_vals'_aux ves acc = (vs, es) ->
+    (exists vs0, split_vals_e ves = (vs0, es) /\ vs = rev vs0 ++ acc).
+Proof.
+  elim => /=.
+  - move => acc vs es.
+    + move => [<- <-]; by eexists; split.
+  - move => e ves' IH acc vs es.
+    destruct (e_to_v_opt e) as [v |] eqn:Hetov.
+    + destruct e as [b | | | |] => //; destruct b => //=.
+      simpl in Hetov; injection Hetov as ->; move => /= Hsplit.
+      apply IH in Hsplit as [vs0 [-> ->]].
+      eexists; split => //=.
+      by rewrite rev_cons -cats1 -catA cat1s.
+    + move => [<- <-].
+      exists nil.
+      split => //.
+      destruct e as [b | | | |] => //; by destruct b.
+Qed.
+
+Lemma split_vals'_aux_spec: forall ves acc vs es vs0,
+    split_vals_e ves = (vs0, es) ->
+    vs = rev vs0 ++ acc ->
+    split_vals'_aux ves acc = (vs, es).
+Proof.
+  elim => /=.
+  - by move => acc vs es vs0 [<- <-] ->.
+  - move => e ves' IH acc vs es vs0 Heq ->.
+    destruct (split_vals_e ves') as [vs' es'] eqn:Hsplit.
+    destruct (e_to_v_opt e) as [v | ] eqn:Hetov.
+    + destruct e as [b | | | |] => //; destruct b => //=.
+      simpl in Hetov; injection Hetov as ->.
+      injection Heq as <- <-.
+      erewrite IH; eauto.
+      by rewrite rev_cons -cats1 -catA cat1s.
+    + destruct e as [b | | | |]; first (destruct b); by injection Heq as <- <-.
+Qed.
+
+Lemma split_vals'_spec: forall ves vs es,
+    split_vals' ves = (vs, es) <->
+    split_vals_e ves = (rev vs, es).
+Proof.
+  move => ves vs es.
+  split; move => Hsplit.
+  - apply split_vals'_aux_impl in Hsplit as [vs0 [Hsplit ->]].
+    by rewrite Hsplit cats0 revK.
+  - eapply split_vals'_aux_spec; eauto.
+    by rewrite cats0 revK.
+Qed.
+
+Function ctx_decompose_aux (ves_acc: (list administrative_instruction) * (list closure_ctx)) {measure (fun '(ves, acc) => ais_measure ves)} : option (list closure_ctx * seq_ctx * option administrative_instruction) :=
+  let '(ves, acc) := ves_acc in
+  match split_vals' ves with
+  | (vs, es) =>
+      match es with
+      | nil => Some (acc, (vs, nil), None)
+      | e :: es' =>
+          match e with
+          | AI_label k ces es =>
+              match acc with
+              | nil => None (* ctx_decompose_aux (es, [:: (empty_frame_ctx, [::Build_label_ctx vs k ces es'])]) *)
+              | (fc, lcs) :: ccs' => ctx_decompose_aux (es, (fc, (Build_label_ctx vs k ces es') :: lcs) :: ccs')
+              end
+          | AI_local k f es =>
+              ctx_decompose_aux (es, (Build_frame_ctx vs k f es', nil) :: acc)
+          | _ => (* In this case, we know that e cannot be const due to a lemma *)
+              Some (acc, (vs, es'), Some e)
+          end
+      end
+  end.
+Proof.
+ (* { move => [ves acc] ves' acc' vs ? e es' k ces es ?? Hsplit ? [? ?]; subst.
+    apply split_vals'_spec, split_vals_inv in Hsplit as ->.
+    rewrite ais_measure_cat ais_measure_cons /ais_measure => /=.
+    by lias.
+  }*)
+  { move => [ves acc] ves' acc' vs ? e es' k ces es ?? Hsplit cc ccs fc lcs ?? [? ?]; subst.
+    apply split_vals'_spec, split_vals_inv in Hsplit as ->.
+    rewrite ais_measure_cat ais_measure_cons /ais_measure => /=.
+    by lias.
+  }
+  { move => [ves acc] ves' acc' [? ?] vs ? e es' k f ??? Hsplit; subst.
+    apply split_vals'_spec, split_vals_inv in Hsplit as ->.
+    rewrite ais_measure_cat ais_measure_cons /ais_measure => /=.
+    by lias.
+  }
+Defined.
+
+Definition ctx_decompose ves := ctx_decompose_aux (ves, nil).
+
+(* Auxiliary definitions for maintaining the canonical decomposition during execution. These avoid the need to
+   invoke split_vals again unless the hole itself is a const *)
+Definition ctx_update_nconst (acc: list closure_ctx) (sctx: seq_ctx) e :=
+  let '(vs, es0) := sctx in
+  match e with
+  | AI_label k ces es =>
+      match acc with
+      | nil => None 
+      | (fc, lcs) :: ccs' => ctx_decompose_aux (es, (fc, (Build_label_ctx vs k ces es0) :: lcs) :: ccs')
+      end
+  | AI_local k f es =>
+      ctx_decompose_aux (es, (Build_frame_ctx vs k f es0, nil) :: acc)
+  | _ => Some (acc, (vs, es0), Some e)
+  end.
+
+Definition ctx_update (acc: list closure_ctx) (sctx: seq_ctx) e :=
+  match e_to_v_opt e with
+  | Some v =>
+      let '(vs, es) := sctx in
+      let '(vs', es') := split_vals' es in
+      match es' with
+      | nil => Some (acc, (vs' ++ [::v] ++ vs, nil), None)
+      | e' :: es'' => ctx_update_nconst acc (vs' ++ [::v] ++ vs, es'') e'
+      end
+  | None => ctx_update_nconst acc sctx e
+  end.
+
+Lemma ctx_decompose_valid_aux: forall ves acc ccs sctx oe,
+    ctx_decompose_aux (ves, acc) = Some (ccs, sctx, oe) ->
+    valid_split sctx oe.
+Proof.
+  move => ves.
+  remember (ais_measure ves) as m.
+  move: Heqm.
+  move: ves.
+  induction m as [m' IH] using (lt_wf_ind).
+  move => ves ? acc ccs sctx oe Hdecomp; subst m'.
+  rewrite ctx_decompose_aux_equation in Hdecomp.
+  destruct (split_vals' ves) as [vs es] eqn:Hsplit.
+  apply split_vals'_spec in Hsplit.
+  destruct es as [ | e es']; first by injection Hdecomp as <- <- <-.
+  destruct e as
+    [ b
+    |
+    | addr
+    | n ces es
+    | n f es
+    ]; simpl in *; try by injection Hdecomp as <- <- <-.
+  - injection Hdecomp as <- <- <- => /=.
+    apply split_vals_nconst in Hsplit.
+    by destruct b.
+  - destruct acc as [ | [fc lcs] ccs'] => //.
+    eapply IH in Hdecomp; eauto; apply split_vals_inv in Hsplit as ->.
+    by rewrite ais_measure_cat ais_measure_cons /ais_measure => /=; lias.
+  - eapply IH in Hdecomp; eauto; apply split_vals_inv in Hsplit as ->.
+    by rewrite ais_measure_cat ais_measure_cons /ais_measure => /=; lias.
+Qed.
+
+Lemma ctx_decompose_valid: forall ves ccs sctx oe,
+    ctx_decompose ves = Some (ccs, sctx, oe) ->
+    valid_split sctx oe.
+Proof.
+  intros.
+  by eapply ctx_decompose_valid_aux; eauto.
+Qed.
+
+Lemma ctx_update_nconst_valid: forall sctx e ccs ccs' sctx' oe,
+    ~ is_const e ->
+    ctx_update_nconst ccs sctx e = Some (ccs', sctx', oe) ->
+    valid_split sctx' oe.
+Proof.
+  move => [vs es] e ccs ccs' [vs' es'] oe Hnconst Hupdate.
+  unfold ctx_update_nconst in Hupdate.
+  destruct e; try injection Hupdate as <- <- <-; subst => //; try by destruct b.
+  (* Label *)
+  - destruct ccs as [ | [fc lcs] ccs0] => //.
+    by apply ctx_decompose_valid_aux in Hupdate.
+  (* Local *)
+  -  by apply ctx_decompose_valid_aux in Hupdate.
+Qed.
+
+Lemma ctx_update_valid: forall sctx e ccs ccs' sctx' oe,
+    ctx_update ccs sctx e = Some (ccs', sctx', oe) ->
+    valid_split sctx' oe.
+Proof.
+  move => [vs es] e ccs ccs' [vs' es'] oe Hupdate.
+  unfold ctx_update in Hupdate.
+  destruct (e_to_v_opt e) as [v | ] eqn:Hetov.
+  - destruct (split_vals' es) as [vs'' es''] eqn:Hsplit.
+    destruct es'' as [ | e0 es'']; try by injection Hupdate as <- <- <-; subst => //.
+    apply split_vals'_spec, split_vals_nconst in Hsplit.
+    by apply ctx_update_nconst_valid in Hupdate => //.
+  - apply ctx_update_nconst_valid in Hupdate => //.
+    by destruct e => //; destruct b.
+Qed.
+
+Lemma ctx_decompose_fill_aux: forall ves acc ccs sctx oe,
+    ctx_decompose_aux (ves, acc) = Some (ccs, sctx, oe) ->
+    ccs ⦃ sctx ⦃ olist oe ⦄ ⦄ = acc ⦃ ves ⦄.
+Proof.
+  move => ves.
+  remember (ais_measure ves) as m.
+  move: Heqm.
+  move: ves.
+  induction m as [m' IH] using (lt_wf_ind).
+  move => ves ? acc ccs sctx oe Hdecomp; subst m'.
+  rewrite ctx_decompose_aux_equation in Hdecomp.
+  destruct (split_vals' ves) as [vs es] eqn:Hsplit.
+  apply split_vals'_spec in Hsplit.
+  destruct es as [ | e es'].
+  - injection Hdecomp as <- <- <- => //=.
+    by apply split_vals_inv in Hsplit as ->.
+  - destruct e as
+      [ b
+      |
+      | addr
+      | n ces es
+      | n f es
+      ]; simpl in *; try by injection Hdecomp as <- <- <- => /=; apply split_vals_inv in Hsplit as ->.
+    (* Label *)
+    + destruct acc as [ | [fc lcs] ccs']; first by inversion Hdecomp => /=.
+      eapply IH in Hdecomp; eauto; apply split_vals_inv in Hsplit as ->; first by rewrite Hdecomp.
+      by rewrite ais_measure_cat ais_measure_cons /ais_measure => /=; lias.
+    (* Local *)
+    + eapply IH in Hdecomp; eauto; apply split_vals_inv in Hsplit as ->; first by rewrite Hdecomp.
+      by rewrite ais_measure_cat ais_measure_cons /ais_measure => /=; lias.
+Qed.
+
+Lemma ctx_decompose_fill_id: forall ves ccs sctx oe,
+    ctx_decompose ves = Some (ccs, sctx, oe) ->
+    ccs ⦃ sctx ⦃ olist oe ⦄ ⦄ = ves.
+Proof.
+  move => ves ccs sctx oe Hdecomp.
+  by apply ctx_decompose_fill_aux in Hdecomp.
+Qed.
+
+Lemma ctx_update_nconst_fill: forall sctx e ccs ccs' sctx' oe,
+    ctx_update_nconst ccs sctx e = Some (ccs', sctx', oe) ->
+    ccs ⦃ sctx ⦃ [::e] ⦄ ⦄ = ccs' ⦃ sctx' ⦃ olist oe ⦄ ⦄.
+Proof.
+  move => [vs es] e ccs ccs' [vs' es'] oe Hupdate.
+  unfold ctx_update_nconst in Hupdate.
+  destruct e => //; try by injection Hupdate as <- <- <-; subst.
+  (* Local *)
+  - destruct ccs as [ | [fc lcs] ccs0] => //.
+    by apply ctx_decompose_fill_aux in Hupdate.
+  - by apply ctx_decompose_fill_aux in Hupdate.
+Qed.
+  
+Lemma ctx_update_fill: forall sctx e ccs ccs' sctx' oe,
+    ctx_update ccs sctx e = Some (ccs', sctx', oe) ->
+    ccs ⦃ sctx ⦃ [::e] ⦄ ⦄ = ccs' ⦃ sctx' ⦃ olist oe ⦄ ⦄.
+Proof.
+  move => [vs es] e ccs ccs' [vs' es'] oe Hupdate.
+  unfold ctx_update in Hupdate.
+  destruct (e_to_v_opt e) as [v | ] eqn:Hetov; last by apply ctx_update_nconst_fill in Hupdate.
+  destruct (split_vals' es) as [vs0 es0] eqn:Hsplit.
+  apply split_vals'_spec, split_vals_inv in Hsplit as ->.
+  destruct es0.
+  - injection Hupdate as <- <- <-; subst; rewrite cats0 => //.
+    destruct e => //; destruct b => //; simpl in Hetov; injection Hetov as -> => /=.
+    f_equal.
+    rewrite cats0 /vs_to_es rev_cat rev_cons -cats1 -catA.
+    by repeat rewrite -v_to_e_cat.
+  - destruct e => //; destruct b => //; simpl in Hetov; injection Hetov as ->.
+    apply ctx_update_nconst_fill in Hupdate.
+    rewrite - Hupdate => /=.
+    f_equal.
+    rewrite /vs_to_es rev_cat rev_cons -cats1 -catA.
+    repeat rewrite -v_to_e_cat.
+    by rewrite -catA.
+Qed.
 
 End EvalContext.
