theories/interpreter_ctx.v
@@ -1,6 +1,6 @@
 (** Proof-carrying interpreter for Wasm, optimised for contexts **)
 
-From Wasm Require Import common properties opsem_properties tactic typing_inversion contexts.
+From Wasm Require Import common properties opsem_properties tactic typing_inversion interpreter_func contexts.
 From Coq Require Import ZArith.BinInt Program.Equality.
 From mathcomp Require Import ssreflect ssrfun ssrnat ssrbool eqtype seq.
 From Wasm Require Export operations host.
@@ -15,17 +15,14 @@ Section Host.
 
 Import EvalContext.
   
-Variable host_function : eqType.
-Let host := host host_function.
-Let cfg_tuple_ctx := @cfg_tuple_ctx host_function.
+Let host := host EvalContext.host_function.
+Let cfg_tuple_ctx := @cfg_tuple_ctx EvalContext.host_function.
 
-Variable host_instance : host.
+Let store_record := store_record EvalContext.host_function.
+Let host_state := host_state EvalContext.host_instance.
 
-Let store_record := store_record host_function.
-Let host_state := host_state host_instance.
-
-Let e_typing := @e_typing host_function.
-Let inst_typing := @inst_typing host_function.
+Let e_typing := @e_typing EvalContext.host_function.
+Let inst_typing := @inst_typing EvalContext.host_function.
 
 Variable host_application_impl : host_state -> store_record -> function_type -> host_function -> seq value ->
                        (host_state * option (store_record * result)).
@@ -33,24 +30,733 @@ Variable host_application_impl : host_state -> store_record -> function_type -> 
 Hypothesis host_application_impl_correct :
   (forall hs s ft hf vs hs' hres, (host_application_impl hs s ft hf vs = (hs', hres)) -> host_application hs s ft hf vs hs' hres).
 
-Definition olist {T: Type} (ot: option T) : list T :=
-  match ot with
-  | Some t => [::t]
-  | None => nil
-  end.
-
-Definition reduce_cfg (hs hs': host_state) (cfg cfg': cfg_tuple_ctx) : Prop :=
+Definition reduce_ctx (hs hs': host_state) (cfg cfg': cfg_tuple_ctx) : Prop :=
   match cfg with
-  | (s, f, cc, e) =>
+  | (s, ccs, sc, oe) =>
       match cfg' with
-      | (s', f', cc', e') => reduce hs s f (cc [[ olist e ]]) hs' s' f' (cc' [[ olist e' ]])
+      | (s', ccs', sc', oe') => reduce hs s empty_frame (ccs ⦃ sc ⦃ olist oe ⦄ ⦄) hs' s' empty_frame (ccs' ⦃ sc' ⦃ olist oe' ⦄ ⦄)
       end
   end.
 
-Definition run_one_step (hs: host_state) (cfg: cfg_tuple_ctx) : {hs' & {cfg' | reduce_cfg hs hs' cfg cfg'}}.
+(*
+Lemma reduce_ctx_reduce (hs hs': host_state) s f s' f' es es':
+  (forall ccs sc oe ccs' sc' oe', ccs ⦃ sc ⦃ olist oe ⦄ ⦄ = es ->
+  ccs' ⦃ sc' ⦃ olist oe' ⦄ ⦄ = es' ->
+  reduce_ctx hs hs' (s, f, ccs, sc, oe) (s', f', ccs', sc', oe')) <->
+  reduce hs s f es hs' s' f' es'.
 Proof.
-  destruct cfg as [[[s f] cc] e].
-  destruct e as [e | ]; last first.
+  split; last by intros; subst.
+  move => Hred.
+  remember (ctx_decompose es) as de.
+  destruct de as [[ccs sc] oe].
+  symmetry in Heqde.
+  remember (ctx_decompose es') as de'.
+  destruct de' as [[ccs' sc'] oe'].
+  symmetry in Heqde'.
+  apply decompose_fill_id in Heqde.
+  apply decompose_fill_id in Heqde'.
+  specialize (Hred _ _ _ _ _ _ Heqde Heqde').
+  unfold reduce_ctx in Hred.
+  by rewrite Heqde Heqde' in Hred.
+Qed.
+*)
+
+Ltac red_ctx_simpl :=
+  repeat lazymatch goal with
+  | _: _ |- reduce _ _ _ (foldl closure_ctx_fill _ _) _ _ _ (foldl closure_ctx_fill _ _) =>
+      apply (list_closure_ctx_eval.(ctx_reduce))
+  | _: _ |- reduce _ _ _ (foldl label_ctx_fill _ _) _ _ _ (foldl label_ctx_fill _ _) =>
+      apply (list_label_ctx_eval.(ctx_reduce))
+  end.
+
+Ltac infer_hole :=
+  repeat lazymatch goal with
+  | |- context C [vs_to_es _] =>
+      rewrite /vs_to_es
+  | _: _ |- ?l ++ _ = ?l ++ _ =>
+      f_equal => //
+  | _: _ |- ?l1 ++ ?l2 = ?x :: ?l2 =>
+      try instantiate (1 := [::x]) => //
+  | _: _ |- ?l1 ++ ?l2 = ?x1 :: ?x2 :: ?l2 =>
+      instantiate (1 := [::x1; x2]) => //
+  | _: _ |- ?l1 ++ ?l2 = ?l3 ++ ?x :: ?l2 =>
+      try instantiate (1 := l3 ++ [::x]); rewrite -catA => //
+  | |- context C [ _ ++ [::] ] =>
+      rewrite cats0
+  | |- context C [v_to_e_list (rev (?l1 ++ ?l2))] =>
+      rewrite rev_cat -v_to_e_cat => //
+  | |- context C [ ( _ ++ _) ++ _ ] =>
+      rewrite -catA
+  end.
+
+Definition run_one_step_ctx (hs: host_state) (cfg: cfg_tuple_ctx) : valid_cfg_ctx cfg -> {hs' & {cfg' | reduce_ctx hs hs' cfg cfg' /\ valid_cfg_ctx cfg'}} + False.
+Proof.
+  move => Hvalid.
+  destruct cfg as [[[s ccs] sc] oe].
+  destruct oe as [e | ]; last first.
+  (* Exitting from contexts *)
+  {
+    unfold valid_cfg_ctx in Hvalid; destruct sc as [vs es]; subst; simpl in *.
+    destruct Hvalid as [? Heq]; move/eqP in Heq; subst es.
+    destruct ccs as [ | [fc lcs] ccs'].
+    { (* entire instruction is const *)
+      right. admit.
+    }
+    { destruct lcs as [ | lc lcs'].
+      (* Exitting a local *)
+      {
+        destruct fc as [lvs lk lf les].
+        destruct (length vs == lk) eqn:Hlen; move/eqP in Hlen.
+        {
+          destruct les as [ | e les'].
+          { (* No instruction in the hole *)
+            left; exists hs, (s, ccs', (vs ++ lvs, nil), None) => /=.
+            split => //.
+            red_ctx_simpl => //.
+            repeat rewrite cats0.
+            eapply r_label with (lh := LH_base (rev lvs) nil) => /=; infer_hole.
+            by apply r_simple, rs_local_const; [ by apply v_to_e_const | by rewrite length_is_size v_to_e_size size_rev ].
+          }
+          { (* e is in the hole *)
+            left; exists hs, (s, ccs', (vs ++ lvs, les'), Some e) => /=.
+            split => //.
+            red_ctx_simpl => //.
+            rewrite cats0.
+            eapply r_label with (lh := LH_base (rev lvs) (e :: les')) => /=; infer_hole.
+            by apply r_simple, rs_local_const; [ by apply v_to_e_const | by rewrite length_is_size v_to_e_size size_rev ].
+          }
+        }
+        (* length doesn't match *)
+        { right. admit. }
+      }
+      (* Exitting a label *)
+      { destruct lc as [lvs lk lces les].
+        destruct les as [ | e les'].
+        { (* No instruction in the hole still *)
+          left; exists hs, (s, (fc, lcs') :: ccs', (vs ++ lvs, nil), None) => /=.
+          split => //.
+          red_ctx_simpl => //.
+          repeat rewrite cats0.
+          eapply r_label with (lh := LH_base (rev (FC_val fc)) (FC_post fc)) => /=; infer_hole.
+          apply r_local => /=.
+          red_ctx_simpl => //=.
+          unfold fmask0, label_ctx_fill => /=.
+          eapply r_label with (lh := LH_base (rev lvs) nil) => /=; infer_hole.
+          apply r_simple, rs_label_const; by apply v_to_e_const.
+        }
+        { (* e is in the hole *)
+          left; exists hs, (s, (fc, lcs') :: ccs', (vs ++ lvs, ), None) => /=.
+          split => //.
+          red_ctx_simpl => //.
+          rewrite cats0.
+          eapply r_label with (lh := LH_base (rev (FC_val fc)) (FC_post fc)) => /=; infer_hole.
+          apply r_local => /=.
+          red_ctx_simpl => //=.
+          unfold fmask0, label_ctx_fill => /=.
+          eapply r_label with (lh := LH_base (rev lvs) (e :: les')) => /=; infer_hole.
+          apply r_simple, rs_label_const; by apply v_to_e_const.
+        }
+      }
+  }
+  { destruct cc as [ | cc ccs]; first exact None.
+    destruct cc as [[fctx lctx] [vs es]].
+    destruct e as [
+      (* AI_basic *) [
+      (* BI_unreachable *) |
+      (* BI_nop *) |
+      (* BI_drop *) |
+      (* BI_select *) |
+      (* BI_block (Tf t1s t2s) es *) [t1s t2s] es |
+      (* BI_loop (Tf t1s t2s) es *) [t1s t2s] es |
+      (* BI_if tf es1 es2 *) tf es1 es2 |
+      (* BI_br j *) j |
+      (* BI_br_if j *) j |
+      (* BI_br_table js j *) js j |
+      (* BI_return *) |
+      (* BI_call j *) j |
+      (* BI_call_indirect j *) j |
+      (* BI_get_local j *) j |
+      (* BI_set_local j *) j |
+      (* BI_tee_local j *) j |
+      (* BI_get_global j *) j |
+      (* BI_set_global j *) j |
+      (* BI_load t [Some (tp, sx)|None] a off *) t [[tp sx]|] a off |
+      (* BI_store t [Some tp|None] a off *) t [tp|] a off |
+      (* BI_current_memory *) |
+      (* BI_grow_memory *) |
+      (* BI_const _ *) |
+      (* BI_unop t op *) t op |
+      (* BI_binop t op *) t op |
+      (* BI_testop [T_i32|T_i64|T_f32|T_f64] testop *) [| | |] testop |
+      (* BI_relop t op *) t op |
+      (* BI_cvtop t2 [CVO_convert|CVO_reinterpret] t1 sx *) t2 [|] t1 sx ] |
+      (* AI_trap *) |
+      (* AI_invoke a *) a |
+      (* AI_label ln les es *) ln les es |
+      (* AI_local ln lf es *) ln lf es ].
+
+    * (* AI_basic BI_unreachable *)
+      apply <<hs, s, f, vs_to_es ves ++ [:: AI_trap]>>'.
+      by apply reduce_unreachable.
+
+    * (* AI_basic BI_nop *)
+      apply <<hs, s, f, vs_to_es ves>>'.
+      by apply reduce_nop.
+
+    * (* AI_basic BI_drop *)
+      destruct ves as [|v ves'] eqn:Heqves.
+      + (* [::] *)
+        apply RS''_error. by apply drop_error.
+      + (* v :: ves' *)
+        apply <<hs, s, f, vs_to_es ves'>>'. by apply reduce_drop.
+
+    * (* AI_basic BI_select *)
+      destruct ves as [|v3 [|v2 [|v1 ves']]];
+        try by (apply RS''_error; apply select_error_size).
+      (* [:: v3, v2, v1 & ves'] *)
+      destruct v3 as [c| | |] eqn:?;
+        try by
+          (apply RS''_error; eapply select_error_i32 with (v3 := v3); subst v3).
+      (* VAL_int32 c *)
+      destruct (c == Wasm_int.int_zero i32m) eqn:?.
+      + (* true *)
+        apply <<hs, s, f, vs_to_es (v2 :: ves')>>'.
+        by apply reduce_select_false.
+      + (* false *)
+        apply <<hs, s, f, vs_to_es (v1 :: ves')>>'.
+        by apply reduce_select_true; clear run_step_aux; lias.
+
+    * (* AI_basic (BI_block (Tf t1s t2s) es) *)
+      destruct (length ves >= length t1s) eqn:?.
+      + (* true *)
+        destruct (split_n ves (length t1s)) as [ves' ves''] eqn:?.
+        remember (AI_label (length t2s) [::] (vs_to_es ves' ++ to_e_list es)) as e'.
+        apply <<hs, s, f, vs_to_es ves'' ++ [:: e']>>'.
+        by subst e'; eapply reduce_block.
+      + (* false *)
+        apply RS''_error.
+        (* TODO should use length in lemmas instead? *)
+        repeat rewrite length_is_size in Heqb.
+        by apply block_error; clear - Heqb; lias.
+
+    * (* AI_basic (BI_loop (Tf t1s t2s) es) *)
+      destruct (length ves >= length t1s) eqn:?.
+      + (* true *)
+        destruct (split_n ves (length t1s)) as [ves' ves''] eqn:?.
+        apply <<hs, s, f, vs_to_es ves''
+          ++ [:: AI_label (length t1s) [:: AI_basic (BI_loop (Tf t1s t2s) es)] (vs_to_es ves' ++ to_e_list es)]
+        >>'.
+        by apply reduce_loop.
+      + (* false *)
+        apply RS''_error.
+        apply loop_error; repeat rewrite -length_is_size; clear run_step_aux; lias.
+
+    * (* AI_basic (BI_if tf es1 es2) *)
+      destruct ves as [|v ves'] eqn:?;
+        try by (apply RS''_error; apply if_error_0).
+      (* v :: ves' *)
+      destruct v as [c| | |] eqn:?;
+        try by (apply RS''_error; eapply if_error_typeof => //).
+      (* VAL_int32 c *)
+      destruct (c == Wasm_int.int_zero i32m) eqn:?.
+      + (* true *)
+        apply <<hs, s, f, vs_to_es ves' ++ [:: AI_basic (BI_block tf es2)]>>'.
+        by eapply reduce_if_false.
+      + (* false *)
+        apply <<hs, s, f, vs_to_es ves' ++ [:: AI_basic (BI_block tf es1)]>>'.
+        by eapply reduce_if_true.
+
+    * (* AI_basic (BI_br j) *)
+      apply break(j, ves).
+      by apply break_br.
+
+    * (* AI_basic (BI_br_if j) *)
+      destruct ves as [|v ves'];
+        try by (apply RS''_error; apply br_if_error_0).
+      (* v :: ves' *)
+      destruct v as [c| | |] eqn:?;
+        try by (apply RS''_error; eapply br_if_error_i32 with (v := v); subst v).
+      (* VAL_int32 c *)
+      destruct (c == Wasm_int.int_zero i32m) eqn:?.
+      ** (* true *)
+         apply <<hs, s, f, vs_to_es ves'>>'.
+         by eapply reduce_br_if_false.
+      ** (* false *)
+         apply <<hs, s, f, vs_to_es ves' ++ [:: AI_basic (BI_br j)]>>'.
+         by eapply reduce_br_if_true; clear run_step_aux; lias.
+
+    * (* AI_basic (BI_br_table js j) *)
+      destruct ves as [|v ves'];
+        try by (apply RS''_error; apply br_table_error_0).
+      (* v :: ves' *)
+      destruct v as [c| | |] eqn:?;
+        try by (apply RS''_error; eapply br_table_error_i32 with (v := v); subst v).
+      remember (Wasm_int.nat_of_uint i32m c) as k.
+      destruct (k < length js) eqn:?.
+      + (* true *)
+        destruct (List.nth_error js k) as [js_at_k|] eqn:?.
+        -- (* Some js_at_k *)
+           apply <<hs, s, f, vs_to_es ves' ++ [::AI_basic (BI_br js_at_k)]>>'.
+           by apply reduce_br_table with (k := k).
+        -- (* None *)
+           apply RS''_error.
+           by apply br_table_error_kth with (k := k) (c := c) (ves' := ves').
+      + (* false *)
+        apply <<hs, s, f, vs_to_es ves' ++ [::AI_basic (BI_br j)]>>'.
+        by apply reduce_br_table_length with (k := k); clear run_step_aux; lias.
+
+    * (* AI_basic BI_return *)
+      apply RS''_return with (rvs := ves).
+      by left => //.
+
+    * (* AI_basic (BI_call j) *)
+      destruct (List.nth_error f.(f_inst).(inst_funcs) j) as [a|] eqn:?.
+      + (* Some a *)
+        apply <<hs, s, f, vs_to_es ves ++ [:: AI_invoke a]>>'.
+        by apply reduce_call.
+      + (* None *)
+        apply RS''_error.
+        by apply call_error.
+
+    * (* AI_basic (BI_call_indirect j) *)
+      destruct ves as [|v ves'] eqn:?;
+        try by (apply RS''_error; apply call_indirect_error_0).
+      (* v :: ves' *)
+      destruct v as [c| | |] eqn:?;
+        try by (apply RS''_error; eapply call_indirect_error_typeof => //).
+      (* VAL_int32 c *)
+      destruct (stab_addr s f (Wasm_int.nat_of_uint i32m c)) as [a|] eqn:?.
+      + (* Some a *)
+        destruct (List.nth_error s.(s_funcs) a) as [cl|] eqn:?.
+        -- (* Some cl *)
+           destruct (stypes s f.(f_inst) j == Some (cl_type cl)) eqn:?.
+           ** (* true *)
+              apply <<hs, s, f, vs_to_es ves' ++ [:: AI_invoke a]>>'.
+              by eapply reduce_call_indirect_success with (cl := cl).
+           ** (* false *)
+              apply <<hs, s, f, vs_to_es ves' ++ [:: AI_trap]>>'.
+              by eapply reduce_call_indirect_failure_1 with (cl := cl) (a := a).
+        -- (* None *)
+           apply RS''_error.
+           by eapply call_indirect_error_ath with (a := a).
+      + (* None *)
+        apply <<hs, s, f, vs_to_es ves' ++ [:: AI_trap]>>'.
+        by eapply reduce_call_indirect_failure_2.
+
+    * (* AI_basic (BI_get_local j) *)
+      destruct (j < length f.(f_locs)) eqn:?.
+      + (* true *)
+        destruct (List.nth_error f.(f_locs) j) as [vs_at_j|] eqn:?.
+        -- (* Some vs_at_j *)
+           apply <<hs, s, f, vs_to_es (vs_at_j :: ves)>>'.
+           by apply reduce_get_local.
+        -- (* None *)
+           apply RS''_error. by apply get_local_error_jth_none.
+      + (* false *)
+        apply RS''_error. by apply get_local_error_length; clear run_step_aux; lias.
+
+    * (* AI_basic (BI_set_local j) *)
+      destruct ves as [|v ves'] eqn:?.
+      + (* [::] *)
+        apply RS''_error. by apply set_local_error_0.
+      + (* v :: ves' *)
+        destruct (j < length f.(f_locs)) eqn:?.
+        -- (* true *)
+           apply <<hs, s, Build_frame (set_nth v f.(f_locs) j v) f.(f_inst), vs_to_es ves'>>'.
+           by eapply reduce_set_local.
+        -- (* false *)
+           apply RS''_error. by eapply set_local_error_length.
+
+    * (* AI_basic (BI_tee_local j) *)
+      destruct ves as [|v ves'] eqn:?.
+      + (* [::] *)
+        apply RS''_error. by apply tee_local_error_0.
+      + (* v :: ves' *)
+        apply <<hs, s, f, vs_to_es (v :: v :: ves') ++ [:: AI_basic (BI_set_local j)]>>'.
+        by eapply reduce_tee_local.
+
+    * (* AI_basic (BI_get_global j) *)
+      destruct (sglob_val s f.(f_inst) j) as [xx|] eqn:?.
+      + (* Some xx *)
+        apply <<hs, s, f, vs_to_es (xx :: ves)>>'.
+        by apply reduce_get_global.
+      + (* None *)
+        apply RS''_error. by apply get_global_error.
+
+    * (* AI_basic (BI_set_global j) *)
+      destruct ves as [|v ves'] eqn:?.
+      + (* [::] *)
+        apply RS''_error. by apply set_global_error_0.
+      + (* v :: ves' *)
+        destruct (supdate_glob s f.(f_inst) j v) as [s'|] eqn:?.
+        -- (* Some s' *)
+           apply <<hs, s', f, vs_to_es ves'>>'.
+           by eapply reduce_set_global => //.
+        -- (* None *)
+           apply RS''_error. by eapply set_global_error_jth.
+
+    * (* AI_basic (BI_load t (Some (tp, sx)) a off) *)
+      (* TODO can this and the next branch be deduped? *)
+      destruct ves as [|v ves'] eqn:?.
+      + (* [::] *)
+        apply RS''_error. by apply load_error_0.
+      + (* v :: ves' *)
+        destruct v as [c| | |] eqn:?;
+          try by (apply RS''_error; eapply load_error_typeof => //).
+        (* VAL_int32 c *)
+        destruct (smem_ind s f.(f_inst)) as [j|] eqn:?.
+        -- (* Some j *)
+           destruct (List.nth_error s.(s_mems) j) as [mem_s_j|] eqn:?.
+           ** (* Some mem_s_j*)
+              destruct (load_packed sx (mem_s_j) (Wasm_int.N_of_uint i32m c) off (tp_length tp) (t_length t)) as [bs|] eqn:?.
+              ++ (* Some bs *)
+                 apply <<hs, s, f, vs_to_es (wasm_deserialise bs t :: ves')>>'.
+                 by apply reduce_load_packed_success with (mem_s_j := mem_s_j) (j := j) (c := c).
+              ++ (* None *)
+                 apply <<hs, s, f, vs_to_es ves' ++ [:: AI_trap]>>'.
+                 by apply reduce_load_packed_failure with (mem_s_j := mem_s_j) (j := j) (c := c).
+           ** (* None*)
+              apply RS''_error. by eapply load_error_jth with (j := j).
+        -- (* None *)
+           apply RS''_error. by eapply load_error_smem_ind.
+
+    * (* AI_basic (BI_load t None a off) *)
+      destruct ves as [|v ves'] eqn:?.
+      + (* [::] *)
+        apply RS''_error. by apply load_error_0.
+      + (* v :: ves' *)
+        destruct v as [c| | |] eqn:?;
+          try by (apply RS''_error; eapply load_error_typeof => //).
+        (* VAL_int32 c *)
+        destruct (smem_ind s f.(f_inst)) as [j|] eqn:?.
+        -- (* Some j *)
+           destruct (List.nth_error s.(s_mems) j) as [mem_s_j|] eqn:?.
+           ** (* Some mem_s_j*)
+              destruct (load (mem_s_j) (Wasm_int.N_of_uint i32m c) off (t_length t)) as [bs|] eqn:?.
+              ++ (* Some bs *)
+                 apply <<hs, s, f, vs_to_es (wasm_deserialise bs t :: ves')>>'.
+                 by apply reduce_load_success
+                   with (c := c) (j := j) (mem_s_j := mem_s_j).
+              ++ (* None *)
+                 apply <<hs, s, f, vs_to_es ves' ++ [:: AI_trap]>>'.
+                 by apply reduce_load_failure
+                   with (c := c) (j := j) (mem_s_j := mem_s_j).
+           ** (* None *)
+              apply RS''_error. by eapply load_error_jth with (j := j).
+        -- (* None *)
+           apply RS''_error. by eapply load_error_smem_ind.
+
+    * (* AI_basic (BI_store t (Some tp) a off) *)
+      (* TODO dedupe with the branch below by matching tp later? *)
+      destruct ves as [|v [|v' ves']] eqn:?;
+        try by (apply RS''_error; apply store_error_size).
+      (* v :: v' :: ves' *)
+      destruct v' as [c| | |] eqn:?;
+        try by (apply RS''_error; eapply store_error_typeof => //).
+      (* VAL_int32 c *)
+      destruct (types_agree t v) eqn:?.
+      + (* true *)
+        destruct (smem_ind s f.(f_inst)) as [j|] eqn:?.
+        -- (* Some j *)
+           destruct (List.nth_error s.(s_mems) j) as [mem_s_j|] eqn:?.
+           ** (* Some mem_s_j *)
+              destruct (store_packed mem_s_j (Wasm_int.N_of_uint i32m c) off (bits v) (tp_length tp)) as [mem'|] eqn:?.
+              ++ (* Some mem' *)
+                 apply <<hs, upd_s_mem s (set_nth mem' s.(s_mems) j mem'), f, vs_to_es ves'>>'.
+                 by eapply reduce_store_packed_success with (mem_s_j := mem_s_j).
+              ++ (* None *)
+                 apply <<hs, s, f, vs_to_es ves' ++ [:: AI_trap]>>'.
+                 by eapply reduce_store_packed_failure with (j := j) (mem_s_j := mem_s_j).
+           ** (* None *)
+              apply RS''_error. by eapply store_error_jth with (j := j).
+        -- (* None *)
+           apply RS''_error. by eapply store_error_smem.
+      + (* false *)
+        apply RS''_error. by apply store_error_types_disagree with (v := v) (c := c) (ves' := ves').
+
+    * (* AI_basic (BI_store t None a off) *)
+      destruct ves as [|v [|v' ves']] eqn:?;
+        try by (apply RS''_error; apply store_error_size).
+      (* v :: v' :: ves' *)
+      destruct v' as [c| | |] eqn:?;
+        try by (apply RS''_error; eapply store_error_typeof => //).
+      (* VAL_int32 c *)
+      destruct (types_agree t v) eqn:?.
+      + (* true *)
+        destruct (smem_ind s f.(f_inst)) as [j|] eqn:?.
+        -- (* Some j *)
+           destruct (List.nth_error s.(s_mems) j) as [mem_s_j|] eqn:?.
+           ** (* Some mem_s_j *)
+              destruct (store mem_s_j (Wasm_int.N_of_uint i32m c) off (bits v) (t_length t)) as [mem'|] eqn:?.
+              ++ (* Some mem' *)
+                 apply <<hs, upd_s_mem s (set_nth mem' s.(s_mems) j mem'), f, vs_to_es ves'>>'.
+                 by eapply reduce_store_success with (mem_s_j := mem_s_j).
+              ++ (* None *)
+                 apply <<hs, s, f, vs_to_es ves' ++ [:: AI_trap]>>'.
+                 by eapply reduce_store_failure with (j := j) (mem_s_j := mem_s_j).
+           ** (* None *)
+              apply RS''_error. by eapply store_error_jth with (j := j).
+        -- (* None *)
+           apply RS''_error. by eapply store_error_smem.
+      + (* false *)
+        apply RS''_error. by apply store_error_types_disagree with (v := v) (c := c) (ves' := ves').
+
+    * (* AI_basic BI_current_memory *)
+      destruct (smem_ind s f.(f_inst)) as [j|] eqn:?.
+      + (* Some j *)
+        destruct (List.nth_error s.(s_mems) j) as [s_mem_s_j|] eqn:?.
+        -- (* Some j *)
+           remember (VAL_int32 (Wasm_int.int_of_Z i32m (Z.of_nat (mem_size s_mem_s_j)))) as v' eqn:?.
+           apply <<hs, s, f, vs_to_es (v' :: ves)>>'.
+           by apply reduce_current_memory with (j := j) (s_mem_s_j := s_mem_s_j).
+        -- (* None *)
+           apply RS''_error. by apply current_memory_error_jth with (j := j).
+      + (* None *)
+        apply RS''_error. by apply current_memory_error_smem => //.
+
+    * (* AI_basic BI_grow_memory *)
+      destruct ves as [|v ves'] eqn:?;
+        try by (apply RS''_error; apply grow_memory_error_0).
+      (* v :: ves' *)
+      destruct v as [c| | |] eqn:?;
+        try by (apply RS''_error; by eapply grow_memory_error_typeof => //).
+      (* VAL_int32 c *)
+      destruct (smem_ind s f.(f_inst)) as [j|] eqn:?.
+      + (* Some j *)
+        destruct (List.nth_error s.(s_mems) j) as [s_mem_s_j|] eqn:Heqsmem.
+        -- (* Some s_mem_s_j *)
+           remember (mem_grow s_mem_s_j (Wasm_int.N_of_uint i32m c)) as mem'.
+           destruct mem' as [mem''|].
+           ** (* Some mem'' *)
+              remember (VAL_int32 (Wasm_int.int_of_Z i32m (Z.of_nat (mem_size s_mem_s_j)))) as v'.
+              remember (upd_s_mem s (set_nth mem'' s.(s_mems) j mem'')) as s'.
+              apply <<hs, s', f, (vs_to_es (v' :: ves'))>>'.
+              by eapply reduce_grow_memory with (j := j) (s_mem_s_j := s_mem_s_j) (mem'' := mem'') => //.
+           ** (* None *)
+              apply <<hs, s, f, vs_to_es (VAL_int32 int32_minus_one :: ves')>>'.
+              by eapply reduce_grow_memory_failure with (j := j) (s_mem_s_j := s_mem_s_j).
+        -- (* None *)
+           apply RS''_error. by eapply grow_memory_error_jth with (j := j).
+      + (* None *)
+        apply RS''_error. by eapply grow_memory_error_smem => //.
+
+    * (* AI_basic (BI_const _) *)
+      by exfalso.
+
+    * (* AI_basic (BI_unop t op) *)
+      destruct ves as [|v ves'].
+      + (* [::] *)
+        apply RS''_error. by apply unop_error.
+      + (* v :: ves' *)
+        apply <<hs, s, f, vs_to_es (app_unop op v :: ves')>>'.
+        by apply reduce_unop.
+
+    * (* AI_basic (BI_binop t op) *)
+      destruct ves as [|v2 [|v1 ves']];
+        try by (apply RS''_error; apply binop_error_size).
+      (* [:: v2, v1 & ves'] *)
+      destruct (app_binop op v1 v2) as [v|] eqn:?.
+      + (* Some v *)
+        apply <<hs, s, f, vs_to_es (v :: ves')>>'.
+        by apply reduce_binop.
+      + (* None *)
+        apply <<hs, s, f, (vs_to_es ves') ++ [:: AI_trap]>>'.
+        by apply reduce_binop_trap.
+
+    * (* AI_basic (BI_testop T_i32 testop) *)
+      destruct ves as [|[c| | |] ves'] eqn:?;
+        try by (apply RS''_error; by eapply testop_i32_error => //).
+      + (* [::] *)
+        apply RS''_error. by apply testop_error_0.
+      + (* VAL_int32 c :: ves' *)
+        apply <<hs, s, f, vs_to_es (VAL_int32 (wasm_bool (@app_testop_i i32t testop c)) :: ves')>>'.
+        by apply reduce_testop_i32.
+
+    * (* AI_basic (BI_testop T_i64 testop) *)
+      (* TODO un-nest this destruct? could make the 'try by' clearer *)
+      destruct ves as [|v ves'].
+      + (* [::] *)
+        apply RS''_error. by apply testop_error_0.
+      + (* v :: ves' *)
+        destruct v as [|c| |];
+          try by (apply RS''_error; by eapply testop_i64_error => //).
+        (* VAL_int64 c *)
+        apply <<hs, s, f, vs_to_es (VAL_int32 (wasm_bool (@app_testop_i i64t testop c)) :: ves')>>'.
+        by eapply reduce_testop_i64.
+
+    * (* AI_basic (BI_testop T_f32 testop) *)
+      apply RS''_error. by apply testop_f32_error.
+
+    * (* AI_basic (BI_testop T_f64 testop) *)
+      apply RS''_error. by apply testop_f64_error.
+
+    * (* AI_basic (BI_relop t op) *)
+      destruct ves as [|v2 [|v1 ves']];
+          try by (apply RS''_error; apply relop_error_size).
+      (* [:: v2, v1 & ves'] *)
+      apply <<hs, s, f, vs_to_es (VAL_int32 (wasm_bool (app_relop op v1 v2)) :: ves')>>'.
+      by apply reduce_relop.
+
+    * (* AI_basic (BI_cvtop t2 CVO_convert t1 sx) *)
+      destruct ves as [|v ves'];
+        try by (apply RS''_error; apply cvtop_error_0).
+      (* v :: ves' *)
+      destruct (types_agree t1 v) eqn:Ht1.
+      + (* true *)
+        destruct (cvt t2 sx v) as [v'|] eqn:Heqv'.
+        -- (* Some v' *)
+           apply <<hs, s, f, vs_to_es (v' :: ves')>>'.
+           by apply reduce_cvtop_success.
+        -- (* None *)
+           apply <<hs, s, f, vs_to_es ves' ++ [::AI_trap]>>'.
+           by apply reduce_cvtop_trap.
+      + (* false *)
+        apply RS''_error. by eapply cvtop_error_types_disagree.
+
+    * (* AI_basic (BI_cvtop t2 CVO_reinterpret t1 sx) *)
+      destruct ves as [|v ves'];
+        try by (apply RS''_error; apply cvtop_error_0).
+      destruct (types_agree t1 v) eqn:?.
+      + (* true *)
+        destruct sx eqn:Heqsx.
+        -- (* Some _ *)
+           apply RS''_error. by eapply cvtop_error_reinterpret_sx.
+        -- (* None *)
+           apply <<hs, s, f, (vs_to_es (wasm_deserialise (bits v) t2 :: ves'))>>'.
+           by apply reduce_reinterpret.
+      + (* false *)
+        apply RS''_error. by eapply cvtop_error_types_disagree.
+
+    * (* AI_trap *)
+      by exfalso.
+
+    * (* AI_invoke a *)
+      destruct (List.nth_error s.(s_funcs) a) as [cl|] eqn:?.
+      + (* Some cl *)
+        destruct cl as [i [t1s t2s] ts es | [t1s t2s] cl'] eqn:?.
+        -- (* FC_func_native i (Tf t1s t2s) ts es *)
+           remember (length t1s) as n eqn:?.
+           remember (length t2s) as m eqn:?.
+           destruct (length ves >= n) eqn:?.
+           ** (* true *)
+              destruct (split_n ves n) as [ves' ves''] eqn:?.
+              remember (n_zeros ts) as zs eqn:?.
+              apply <<hs, s, f, vs_to_es ves'' ++ [::
+                AI_local
+                m
+                (Build_frame (rev ves' ++ zs) i)
+                [::AI_basic (BI_block (Tf [::] t2s) es)]
+              ]>>'.
+              by eapply reduce_invoke_native with (n := n) (ts := ts) (t1s := t1s).
+           ** (* false *)
+              apply RS''_error.
+              by eapply invoke_func_native_error_n with
+                (n := n) (t1s := t1s) (t2s := t2s) (i := i) (ts := ts) (es := es).
+        -- (* FC_func_host (Tf t1s t2s) cl' *)
+           remember (length t1s) as n eqn:?.
+           remember (length t2s) as m eqn:?.
+           destruct (length ves >= n) eqn:?.
+           ** (* true *)
+              destruct (split_n ves n) as [ves' ves''] eqn:?.
+              destruct (host_application_impl hs s (Tf t1s t2s) cl' (rev ves')) as [hs' [[s' rves]|]] eqn:?.
+              ++ (* (hs', Some (s', rves)) *)
+                 apply <<hs', s', f, vs_to_es ves'' ++ (result_to_stack rves)>>'.
+                 by eapply reduce_invoke_host_success with
+                   (n := n) (t1s := t1s) (t2s := t2s) (cl' := cl') (ves' := ves').
+              ++ (* (hs', None) *)
+                 apply <<hs', s, f, vs_to_es ves ++ [::AI_invoke a]>>'.
+                 by eapply reduce_invoke_host_diverge with
+                   (n := n) (t1s := t1s) (t2s := t2s) (cl' := cl') (ves' := ves') (ves'' := ves'') => //.
+           ** (* false *)
+              apply RS''_error.
+              by eapply invoke_func_host_error_n with
+                (n := n) (t1s := t1s) (t2s := t2s) (cl' := cl').
+      + (* None *)
+        apply RS''_error. by apply invoke_host_error_ath.
+
+    * (* AI_label ln les es *)
+      destruct (es_is_trap es) eqn:?.
+      + (* true *)
+        apply <<hs, s, f, vs_to_es ves ++ [::AI_trap]>>'.
+        by apply reduce_label_trap.
+      + (* false *)
+        destruct (const_list es) eqn:?.
+        -- (* true *)
+           apply <<hs, s, f, vs_to_es ves ++ es>>'.
+           by apply reduce_label_const.
+        -- (* false *)
+          assert (run_step_measure es < S (run_one_step_measure (AI_label ln les es)))%coq_nat as Hmeasure.
+          { simpl. by rewrite run_step_measure_eq; lias. }
+          specialize (run_step_aux hs s f es Hmeasure).
+          destruct run_step_aux as
+             [ Hv | Herr | n bvs H | rvs H | hs' s' f' es'] eqn:?.
+           ** (* RS'_value hs s f Hv *)
+              exfalso. by apply const_trap_contradiction with (es := es).
+           ** (* RS'_error hs Herr *)
+              apply RS''_error.
+              by apply label_error_rec.
+           ** (* RS'_break hs s f es n bvs *)
+              destruct n as [|n].
+              ++ (* 0 *)
+                 destruct (length bvs >= ln) eqn:?.
+                 --- (* true *)
+                     apply <<hs, s, f, vs_to_es ((take ln bvs) ++ ves) ++ les>>'.
+                     by apply reduce_label_break_rec.
+                 --- (* false *)
+                     apply RS''_error.
+                     by apply label_error_break_rec with (bvs := bvs).
+              ++ (* n.+1 *)
+                 apply break(n, bvs).
+                 by apply label_break_rec.
+           ** (* RS'_return hs s f es rvs H *)
+              apply RS''_return with (rvs := rvs).
+              (* TODO move into a lemma? *)
+              right. destruct H as [i [lh H]].
+              by exists ln, les, es, i, lh => //.
+           ** (* RS'_normal hs s f es hs' s' f' es' *)
+              apply <<hs', s', f', vs_to_es ves ++ [:: AI_label ln les es']>>'.
+              by apply reduce_label_rec.
+
+    * (* AI_local ln lf es *)
+      destruct (es_is_trap es) eqn:?.
+      + (* true *)
+        apply <<hs, s, f, vs_to_es ves ++ [::AI_trap]>>'.
+        by apply reduce_local_trap.
+      + (* false *)
+        destruct (const_list es) eqn:?.
+        -- (* true *)
+           destruct (length es == ln) eqn:?.
+           ** (* true *)
+              apply <<hs, s, f, vs_to_es ves ++ es>>'.
+              by apply reduce_local_const.
+           ** (* false *)
+              apply RS''_error.
+              by apply local_error_const_len.
+        -- (* false *)
+           assert (run_step_measure es < S (run_one_step_measure (AI_local ln lf es)))%coq_nat as Hmeasure.
+           { simpl. by rewrite run_step_measure_eq; lias. }
+           specialize (run_step_aux hs s lf es Hmeasure).
+           destruct run_step_aux as
+             [ Hv | Herr | n bvs | rvs H | hs' s' f' es'] eqn:?; clear Hmeasure.
+           ** (* RS'_value hs s f Hv *)
+              exfalso. by apply const_trap_contradiction with (es := es).
+           ** (* RS'_error hs Herr *)
+              apply RS''_error.
+              by apply local_error_rec.
+           ** (* RS'_break hs s f es n bvs *)
+              apply RS''_error.
+              by apply local_error_break_rec with (n := n) (bvs := bvs).
+           ** (* RS'_return hs s f es rvs H *)
+              destruct (length rvs >= ln) eqn:?.
+              ++ (* true *)
+                 apply <<hs, s, f, vs_to_es (take ln rvs ++ ves)>>'.
+                 by apply reduce_local_return_rec.
+              ++ (* false *)
+                 apply RS''_error.
+                 apply local_return_error with (rvs := rvs) => //.
+           ** (* RS'_normal hs s f es hs' s' f' es' *)
+              apply <<hs', s', f, vs_to_es ves ++ [:: AI_local ln f' es']>>'.
+              by apply reduce_local_rec.
 Defined.
 
 End Host.
